Add const right

dimsum/iris/combinators.v
@@ -753,6 +753,25 @@ Section link.
     - iIntros ([[[??]?]?] ?). simplify_eq/=. by iLeft.
   Qed.
 
+  Definition tgt_link_run_right_constP R {m1 m2 : mod_trans (io_event EV)}
+    (Π : option (io_event EV) → link_case EV * S * m_state m1 * m_state m2 → iProp Σ)
+    (γ_s γ_σ1: gname) : option (io_event EV) → m_state m2 → iProp Σ :=
+    λ κ σ2', (∀ s σ1, γ_s ⤳ s -∗ γ_σ1 ⤳ σ1 -∗ tgt_link_run_rightP R Π s σ1 κ σ2')%I.
+
+  Lemma sim_tgt_link_run_right_const R m1 m2 s σ1 σ2 γ_s γ_σ1 Π :
+    γ_s ⤳@{S} - -∗
+    γ_σ1 ⤳@{m_state m1} - -∗
+    (γ_s ⤳ s -∗ γ_σ1 ⤳ σ1 -∗ σ2 ≈{m2}≈>ₜ tgt_link_run_right_constP R Π γ_s γ_σ1) -∗
+    (MLFRun (Some SPRight), s, σ1, σ2) ≈{link_trans R m1 m2}≈>ₜ Π.
+  Proof.
+    iIntros "Hγ_s Hγ_σ1 Hsim".
+    iMod (mstate_var_split γ_s with "Hγ_s") as "[??]".
+    iMod (mstate_var_split γ_σ1 with "Hγ_σ1") as "[??]".
+    iApply sim_tgt_link_run_right. iSpecialize ("Hsim" with "[$] [$]").
+    iApply (sim_gen_wand with "Hsim"). iIntros (??) "Hsim".
+    iApply ("Hsim" with "[$] [$]").
+  Qed.
+
   Definition tgt_link_recv_rightP R {m1 m2 : mod_trans (io_event EV)}
     (Π : option (io_event EV) → link_case EV * S * m_state m1 * m_state m2 → iProp Σ)
     (s : S) (σ1 : m_state m1) e : option (io_event EV) → m_state m2 → iProp Σ :=
@@ -778,4 +797,69 @@ Section link.
     - inv_all @link_filter. iRight. iSplit!. by iApply "Hsim".
     - by iLeft.
   Qed.
+
+  Definition tgt_link_recv_right_constP R {m1 m2 : mod_trans (io_event EV)}
+    (Π : option (io_event EV) → link_case EV * S * m_state m1 * m_state m2 → iProp Σ)
+    (γ_s γ_σ1 γ_e : gname) : option (io_event EV) → m_state m2 → iProp Σ :=
+    λ κ σ2', (∀ s σ1 e, γ_s ⤳ s -∗ γ_σ1 ⤳ σ1 -∗ γ_e ⤳ e -∗ tgt_link_recv_rightP R Π s σ1 e κ σ2')%I.
+
+  Lemma sim_tgt_link_recv_right_const R m1 m2 s σ1 σ2 e γ_s γ_σ1 γ_e Π :
+    γ_s ⤳@{S} - -∗
+    γ_σ1 ⤳@{m_state m1} - -∗
+    γ_e ⤳@{EV}- -∗
+    (γ_s ⤳ s -∗ γ_σ1 ⤳ σ1 -∗ γ_e ⤳ e -∗ σ2 ≈{m2}≈>ₜ tgt_link_recv_right_constP R Π γ_s γ_σ1 γ_e) -∗
+    (MLFRecv SPRight e, s, σ1, σ2) ≈{link_trans R m1 m2}≈>ₜ Π.
+  Proof.
+    iIntros "Hγ_s Hγ_σ1 Hγ_e Hsim".
+    iMod (mstate_var_split γ_s with "Hγ_s") as "[??]".
+    iMod (mstate_var_split γ_σ1 with "Hγ_σ1") as "[??]".
+    iMod (mstate_var_split γ_e with "Hγ_e") as "[??]".
+    iApply sim_tgt_link_recv_right. iSpecialize ("Hsim" with "[$] [$] [$]").
+    iApply (sim_gen_wand with "Hsim"). iIntros (??) "Hsim".
+    iApply ("Hsim" with "[$] [$] [$]").
+  Qed.
+
+  Definition tgt_link_right_constP R {m1 m2 : mod_trans (io_event EV)}
+    (Π : option (io_event EV) → link_case EV * S * m_state m1 * m_state m2 → iProp Σ)
+    (γ_s γ_σ1 γ_oe : gname) : option (io_event EV) → m_state m2 → iProp Σ :=
+    λ κ σ2',
+      (∀ s σ1 oe,
+         γ_s ⤳ s -∗ γ_σ1 ⤳ σ1 -∗ γ_oe ⤳ oe -∗
+         match oe with
+         | Some e => tgt_link_recv_rightP R Π s σ1 e κ σ2'
+         | None => tgt_link_run_rightP R Π s σ1 κ σ2'
+         end)%I.
+
+  Lemma sim_tgt_link_right_const_recv γ_s γ_σ1 γ_oe R m1 m2 s σ1 σ2 e Π :
+    γ_s ⤳@{S} - -∗
+    γ_σ1 ⤳@{m_state m1} - -∗
+    γ_oe ⤳@{option EV}- -∗
+    (γ_s ⤳ s -∗ γ_σ1 ⤳ σ1 -∗ γ_oe ⤳ Some e -∗ σ2 ≈{m2}≈>ₜ tgt_link_right_constP R Π γ_s γ_σ1 γ_oe) -∗
+    (MLFRecv SPRight e, s, σ1, σ2) ≈{link_trans R m1 m2}≈>ₜ Π.
+  Proof.
+    iIntros "Hγ_s Hγ_σ1 Hγ_oe Hsim".
+    iMod (mstate_var_split γ_s with "Hγ_s") as "[??]".
+    iMod (mstate_var_split γ_σ1 with "Hγ_σ1") as "[??]".
+    iMod (mstate_var_split γ_oe with "Hγ_oe") as "[??]".
+    iApply sim_tgt_link_recv_right. iSpecialize ("Hsim" with "[$] [$] [$]").
+    iApply (sim_gen_wand with "Hsim"). iIntros (??) "Hsim".
+    iApply ("Hsim" with "[$] [$] [$]").
+  Qed.
+
+  Lemma sim_tgt_link_right_const_run γ_s γ_σ1 γ_oe R m1 m2 s σ1 σ2 Π :
+    γ_s ⤳@{S} - -∗
+    γ_σ1 ⤳@{m_state m1} - -∗
+    γ_oe ⤳@{option EV}- -∗
+    (γ_s ⤳ s -∗ γ_σ1 ⤳ σ1 -∗ γ_oe ⤳ (@None EV) -∗ σ2 ≈{m2}≈>ₜ tgt_link_right_constP R Π γ_s γ_σ1 γ_oe) -∗
+    (MLFRun (Some SPRight), s, σ1, σ2) ≈{link_trans R m1 m2}≈>ₜ Π.
+  Proof.
+    iIntros "Hγ_s Hγ_σ1 Hγ_oe Hsim".
+    iMod (mstate_var_split γ_s with "Hγ_s") as "[??]".
+    iMod (mstate_var_split γ_σ1 with "Hγ_σ1") as "[??]".
+    iMod (mstate_var_split γ_oe with "Hγ_oe") as "[??]".
+    iApply sim_tgt_link_run_right. iSpecialize ("Hsim" with "[$] [$] [$]").
+    iApply (sim_gen_wand with "Hsim"). iIntros (??) "Hsim".
+    iApply ("Hsim" with "[$] [$] [$]").
+  Qed.
+
 End link.
